secrefstar/MST.Repr.fst
@@ -7,13 +7,16 @@ open FStar.Preorder
 open FStar.Monotonic.Heap
 open FStar.Ghost
 
+open Free
+module G = GuardedDMFree
+
 module W = FStar.Monotonic.Witnessed
 
 (**
   File structured as follows:
   0. Prerequisties about heap and references
   1. Spec monad
-  2. Free monad
+  2. Free monad (instantiation of lib's two-channel free monad)
   3. Define theta and proofs that is a lax morphism
   4. Define Dijkstra Monad
 **)
@@ -60,37 +63,33 @@ let (⊑) #heap #a wp1 wp2 = st_stronger heap a wp2 wp1
 
 (** ** START Section 2: free monad **)
 
+(** The MST commands, as indexed command types for lib's free monad.
+    The commands with Type0 results go on the first channel (summed with
+    the guard commands of lib.GuardedDMFree, which play the role the old
+    PartialCall constructor played); get_heap, whose result erased heap
+    lives in Type u#1, goes on the second channel, whose index universe is
+    independent of the first channel's. *)
 noeq
-type free (a:Type u#a) : Type u#(max 1 a) =
-| Read : #b:Type0 -> #rel: preorder b -> r: mref b rel -> cont:(b -> free a) -> free a
-| Write : #b:Type0 -> #rel: preorder b -> r: mref b rel -> v:b -> cont:free a -> free a
-| Alloc : #b:Type0 -> #rel: preorder b -> init: b -> cont:(mref b rel -> free a) -> free a
-| Witness : p:heap_predicate_stable -> cont:(unit -> free a) -> free a
-| Recall : p:heap_predicate_stable -> cont:(unit -> free a) -> free a
+type mst_cmds : Type0 -> Type u#1 =
+| CRead    : #b:Type0 -> #rel:preorder b -> mref b rel -> mst_cmds b
+| CWrite   : #b:Type0 -> #rel:preorder b -> mref b rel -> b -> mst_cmds unit
+| CAlloc   : #b:Type0 -> #rel:preorder b -> b -> mst_cmds (mref b rel)
+| CWitness : heap_predicate_stable -> mst_cmds unit
+| CRecall  : heap_predicate_stable -> mst_cmds unit
 
-| GetHeap : cont:(erased heap -> free a) -> free a
+noeq
+type heap_cmds : Type u#1 -> Type u#1 =
+| CGetHeap : heap_cmds (erased heap)
 
-| PartialCall : (pre:pure_pre) -> cont:((squash pre) -> free a) -> free a
-| Return : a -> free a
+(** The carrier: lib's two-channel free monad. *)
+let free (a:Type u#a) : Type u#(max 2 a) =
+  Free.free (cmd_sum G.guard_cmd mst_cmds) heap_cmds a
 
 let free_return (a:Type u#a) (x:a) : free a =
-  Return x
+  Free.free_return x
 
-let rec free_bind
-  (#a:Type u#a)
-  (#b:Type u#b)
-  (l : free a)
-  (k : a -> free b) :
-  free b =
-  match l with
-  | Return x -> k x
-  | Read r cont -> Read r (fun x -> free_bind (cont x) k)
-  | Write r v cont -> Write r v (free_bind cont k)
-  | Alloc init cont -> Alloc init (fun x -> free_bind (cont x) k)
-  | Witness pred cont -> Witness pred (fun _ -> free_bind (cont ()) k)
-  | Recall pred cont -> Recall pred (fun _ -> free_bind (cont ()) k)
-  | PartialCall pre fnc -> PartialCall pre (fun _ -> free_bind (fnc ()) k)
-  | GetHeap cont -> GetHeap (fun h -> free_bind (cont h) k)
+let free_bind (#a:Type u#a) (#b:Type u#b) (l:free a) (k:a -> free b) : free b =
+  Free.free_bind l k
 
 (** ** END Section 2: free monad **)
 
@@ -121,7 +120,6 @@ let write_wp (#a:Type) (#rel:preorder a) (r:mref a rel) (v:a)
     (forall a. h0 `heap_rel` (upd h0 r v) /\ write_post r v h0 a (upd h0 r v) ==> p a (upd h0 r v))
 
 let alloc_post #a #rel init h0 (r:mref a rel) h1 : Type0 =
-  (addr_of r) `addr_unused_in` h0 /\
   fresh r h0 h1 /\ modifies Set.empty h0 h1 /\ sel h1 r == init /\
   h1 == upd h0 r init /\ is_mm r == false /\
   addr_of r == next_addr h0 /\
@@ -144,24 +142,32 @@ unfold
 let get_heap_wp : st_mwp_h heap (erased heap) =
   fun p h0 -> p (hide h0) h0
 
+(** State-based WP of a first-channel command (guards + mst_cmds).
+    (Note: destructing the command inside a `Call1` pattern trips universe
+    inference, so the dispatch lives in a helper where `r` is a regular
+    binder.) *)
+let cmd_st_wp (#r:Type0) (op:cmd_sum G.guard_cmd mst_cmds r) : st_mwp_h heap r =
+  match op with
+  | CmdL (G.GCmd pre)          -> partial_call_wp pre
+  | CmdR (CRead #b #rel r)     -> read_wp r
+  | CmdR (CWrite #b #rel r v)  -> write_wp r v
+  | CmdR (CAlloc #b #rel init) -> alloc_wp #b #rel init
+  | CmdR (CWitness pred)       -> witness_wp pred
+  | CmdR (CRecall pred)        -> recall_wp pred
+
+(** State-based WP of a second-channel command (get_heap). *)
+let heap_cmd_st_wp (#r:Type u#1) (op:heap_cmds r) : st_mwp_h heap r =
+  match op with
+  | CGetHeap -> get_heap_wp
+
 val theta : #a:Type u#a -> free a -> st_mwp_h heap a
 let rec theta #a m =
   match m with
   | Return x -> st_return heap _ x
-  | PartialCall pre k ->
-      st_bind_wp heap _ _ (partial_call_wp pre) (fun r -> theta (k r))
-  | GetHeap k ->
-      st_bind_wp heap _ _ get_heap_wp (fun r -> theta (k r))
-  | Read r k ->
-      st_bind_wp heap _ _ (read_wp r) (fun r -> theta (k r))
-  | Write r v k ->
-      st_bind_wp heap _ _ (write_wp r v) (fun _ -> theta k)
-  | Alloc init k ->
-      st_bind_wp heap _ _ (alloc_wp init) (fun r -> theta (k r))
-  | Witness pred k ->
-      st_bind_wp heap _ _ (witness_wp pred) (fun r -> theta (k r))
-  | Recall pred k ->
-      st_bind_wp heap _ _ (recall_wp pred) (fun r -> theta (k r))
+  | Call1 op k ->
+      st_bind_wp heap _ _ (cmd_st_wp op) (fun r -> theta (k r))
+  | Call2 op k ->
+      st_bind_wp heap _ _ (heap_cmd_st_wp op) (fun r -> theta (k r))
 
 let lemma_theta_is_monad_morphism_ret (v:'a) :
   Lemma (theta (free_return 'a v) == st_return heap 'a v) by (compute ()) = ()
@@ -174,12 +180,12 @@ let rec lemma_theta_is_lax_morphism_bind
     (theta (free_bind m f) ⊑ st_bind_wp heap a b (theta m) (fun x -> theta (f x))) =
   match m with
   | Return x -> ()
-  | Read r k ->
+  | Call1 op k ->
     begin
       calc (⊑) {
-        theta (free_bind (Read r k) f) ;
+        theta (free_bind (Call1 op k) f) ;
         ⊑ {}
-        st_bind_wp heap _ _ (read_wp r) (fun r -> theta (free_bind (k r) f)) ;
+        st_bind_wp heap _ _ (cmd_st_wp op) (fun r -> theta (free_bind (k r) f)) ;
         ⊑ {
           let lhs = fun r -> theta (free_bind (k r) f) in
           let rhs = fun x -> st_bind_wp heap _ _ (theta (k x)) (fun x -> theta (f x)) in
@@ -187,29 +193,17 @@ let rec lemma_theta_is_lax_morphism_bind
             lemma_theta_is_lax_morphism_bind (k x) f
           end
         }
-        st_bind_wp heap _ _ (read_wp r) (fun x -> st_bind_wp heap _ _ (theta (k x)) (fun x -> theta (f x))) ;
+        st_bind_wp heap _ _ (cmd_st_wp op) (fun x -> st_bind_wp heap _ _ (theta (k x)) (fun x -> theta (f x))) ;
         ⊑ {}
-        st_bind_wp heap a b (theta (Read r k)) (fun x -> theta (f x)) ;
+        st_bind_wp heap a b (theta (Call1 op k)) (fun x -> theta (f x)) ;
       }
     end
-  | Write r v k ->
+  | Call2 op k ->
     begin
       calc (⊑) {
-        theta (free_bind (Write r v k) f) ;
+        theta (free_bind (Call2 op k) f) ;
         ⊑ {}
-        st_bind_wp heap _ _ (write_wp r v) (fun _ -> theta (free_bind k f)) ;
-        ⊑ { lemma_theta_is_lax_morphism_bind k f }
-        st_bind_wp heap _ _ (write_wp r v) (fun _ -> st_bind_wp heap _ _ (theta k) (fun x -> theta (f x))) ;
-        ⊑ {}
-        st_bind_wp heap a b (theta (Write r v k)) (fun x -> theta (f x)) ;
-      }
-    end
-  | Alloc init k ->
-    begin
-      calc (⊑) {
-        theta (free_bind (Alloc init k) f) ;
-        ⊑ {}
-        st_bind_wp heap _ _ (alloc_wp init) (fun r -> theta (free_bind (k r) f)) ;
+        st_bind_wp heap _ _ (heap_cmd_st_wp op) (fun r -> theta (free_bind (k r) f)) ;
         ⊑ {
           let lhs = fun r -> theta (free_bind (k r) f) in
           let rhs = fun x -> st_bind_wp heap _ _ (theta (k x)) (fun x -> theta (f x)) in
@@ -217,78 +211,9 @@ let rec lemma_theta_is_lax_morphism_bind
             lemma_theta_is_lax_morphism_bind (k x) f
           end
         }
-        st_bind_wp heap _ _ (alloc_wp init) (fun x -> st_bind_wp heap _ _ (theta (k x)) (fun x -> theta (f x))) ;
+        st_bind_wp heap _ _ (heap_cmd_st_wp op) (fun x -> st_bind_wp heap _ _ (theta (k x)) (fun x -> theta (f x))) ;
         ⊑ {}
-        st_bind_wp heap a b (theta (Alloc init k)) (fun x -> theta (f x)) ;
-      }
-    end
-  | Witness pred k -> begin
-    calc (⊑) {
-      theta (free_bind (Witness pred k) f);
-      ⊑ {}
-      st_bind_wp heap unit b (witness_wp pred) (fun r -> theta (free_bind (k r) f));
-      ⊑ {
-          let lhs = fun r -> theta (free_bind (k r) f) in
-          let rhs = fun r -> st_bind_wp heap a b (theta (k r)) (fun x -> theta (f x)) in
-          introduce forall r. lhs r ⊑ rhs r with begin
-            lemma_theta_is_lax_morphism_bind #a #b (k r) f
-          end
-          }
-      st_bind_wp heap unit b (witness_wp pred) (fun r -> st_bind_wp heap a b (theta (k r)) (fun x -> theta (f x)));
-      ⊑ {}
-      st_bind_wp heap a b (theta (Witness pred k)) (fun x -> theta (f x));
-    }
-  end
-  | Recall pred k -> begin
-    calc (⊑) {
-      theta (free_bind (Recall pred k) f);
-      ⊑ {}
-      st_bind_wp heap unit b (recall_wp pred) (fun r -> theta (free_bind (k r) f));
-      ⊑ {
-          let lhs = fun r -> theta (free_bind (k r) f) in
-          let rhs = fun r -> st_bind_wp heap a b (theta (k r)) (fun x -> theta (f x)) in
-          introduce forall r. lhs r ⊑ rhs r with begin
-            lemma_theta_is_lax_morphism_bind #a #b (k r) f
-          end
-          }
-      st_bind_wp heap unit b (recall_wp pred) (fun r -> st_bind_wp heap a b (theta (k r)) (fun x -> theta (f x)));
-      ⊑ {}
-      st_bind_wp heap a b (theta (Recall pred k)) (fun x -> theta (f x));
-    }
-  end
-  | PartialCall pre k -> begin
-    calc (⊑) {
-      theta (free_bind (PartialCall pre k) f);
-      ⊑ {}
-      st_bind_wp heap (squash pre) b (partial_call_wp pre) (fun r -> theta (free_bind (k r) f));
-      ⊑ {
-          let lhs = fun r -> theta (free_bind (k r) f) in
-          let rhs = fun r -> st_bind_wp heap a b (theta (k r)) (fun x -> theta (f x)) in
-          introduce forall (r:squash pre). lhs r ⊑ rhs r with begin
-            lemma_theta_is_lax_morphism_bind #a #b (k r) f
-          end
-          }
-      st_bind_wp heap (squash pre) b (partial_call_wp pre) (fun r -> st_bind_wp heap a b (theta (k r)) (fun x -> theta (f x)));
-      ⊑ {}
-      st_bind_wp heap a b (theta (PartialCall pre k)) (fun x -> theta (f x));
-    }
-  end
-  | GetHeap k ->
-    begin
-      calc (⊑) {
-        theta (free_bind (GetHeap k) f) ;
-        ⊑ {}
-        st_bind_wp heap _ _ get_heap_wp (fun r -> theta (free_bind (k r) f)) ;
-        ⊑ {
-          let lhs = fun r -> theta (free_bind (k r) f) in
-          let rhs = fun x -> st_bind_wp heap _ _ (theta (k x)) (fun x -> theta (f x)) in
-          introduce forall x. lhs x ⊑ rhs x with begin
-            lemma_theta_is_lax_morphism_bind (k x) f
-          end
-        }
-        st_bind_wp heap _ _ get_heap_wp (fun x -> st_bind_wp heap _ _ (theta (k x)) (fun x -> theta (f x))) ;
-        ⊑ {}
-        st_bind_wp heap a b (theta (GetHeap k)) (fun x -> theta (f x)) ;
+        st_bind_wp heap a b (theta (Call2 op k)) (fun x -> theta (f x)) ;
       }
     end
 #pop-options
@@ -324,24 +249,24 @@ let mst_subcomp
   v
 
 let partial_return (pre:pure_pre) : mst (squash pre) (partial_call_wp pre) =
-  PartialCall pre (Return)
+  Call1 (CmdL (G.GCmd pre)) Return
 
 let mst_read (#a:Type) (#rel:preorder a) (r:mref a rel) : mst a (read_wp r) =
-  Read r Return
+  Call1 (CmdR (CRead r)) Return
 
 let mst_write (#a:Type) (#rel:preorder a) (r:mref a rel) (v:a) : mst unit (write_wp r v) =
-  Write r v (Return ())
+  Call1 (CmdR (CWrite r v)) Return
 
 let mst_alloc (#a:Type) (#rel:preorder a) (init:a) : mst (mref a rel) (alloc_wp init) =
-  Alloc init Return
+  Call1 (CmdR (CAlloc init)) Return
 
 let mst_witness (pred:heap_predicate_stable) : mst unit (witness_wp pred) =
-  Witness pred Return
+  Call1 (CmdR (CWitness pred)) Return
 
 let mst_recall (pred:heap_predicate_stable) : mst unit (recall_wp pred) =
-  Recall pred Return
+  Call1 (CmdR (CRecall pred)) Return
 
 let mst_get_heap : mst (erased heap) get_heap_wp =
-  GetHeap Return
+  Call2 CGetHeap Return
 
 (** ** END Section 4: Dijkstra Monad **)
